theories/Nominal.v
@@ -6,9 +6,9 @@ Class Support A := support: A → NameSet.
 
 Section Nominal.
   Context (X: Type) `{PermT X}.
-
+  
   Class Nominal `{Spt: Support X}: Prop := {
-    nperm :: PermT X;
+    nperm :> PermT X;
     support_spec: ∀ (x: X) (a b: Name),
       a ∉ (support x) → b ∉ (support x) → ⟨a,b⟩ • x ≡@{X} x
 }.
